processor: update Kami that initializes program by normal memory load; proof structure changed along with this change.

processor/src/KamiProc.v
@@ -13,32 +13,14 @@ Set Implicit Arguments.
 Section Parametrized.
   Variables addrSize iaddrSize fifoSize instBytes dataBytes rfIdx: nat.
 
-  (* External abstract ISA: decoding and execution *)
-  Variables (getOptype: OptypeT instBytes)
-            (getLdDst: LdDstT instBytes rfIdx)
-            (getLdAddr: LdAddrT addrSize instBytes)
-            (getLdSrc: LdSrcT instBytes rfIdx)
-            (calcLdAddr: LdAddrCalcT addrSize dataBytes)
-            (getStAddr: StAddrT addrSize instBytes)
-            (getStSrc: StSrcT instBytes rfIdx)
-            (calcStAddr: StAddrCalcT addrSize dataBytes)
-            (getStVSrc: StVSrcT instBytes rfIdx)
-            (getSrc1: Src1T instBytes rfIdx)
-            (getSrc2: Src2T instBytes rfIdx)
-            (getDst: DstT instBytes rfIdx)
-            (exec: ExecT iaddrSize instBytes dataBytes)
-            (getNextPc: NextPcT iaddrSize instBytes dataBytes rfIdx)
-            (alignAddr: AlignAddrT addrSize)
-            (isMMIO: IsMMIOT addrSize).
+  Variables (fetch: AbsFetch instBytes dataBytes)
+            (dec: AbsDec addrSize instBytes dataBytes rfIdx)
+            (exec: AbsExec iaddrSize instBytes dataBytes rfIdx)
+            (ammio: AbsMMIO addrSize).
 
   Variable (init: ProcInit iaddrSize dataBytes rfIdx).
 
-  Definition pprocInl :=
-    scmmInl getOptype getLdDst getLdAddr getLdSrc calcLdAddr
-            getStAddr getStSrc calcStAddr getStVSrc
-            getSrc1 getSrc2 getDst exec getNextPc alignAddr
-            isMMIO init.
-
+  Definition pprocInl := scmmInl fetch dec exec ammio init.
   Definition pproc := projT1 pprocInl.
 
   (** The auxiliary hardware state; this is for manipulating hardware state
@@ -52,21 +34,24 @@ Section Parametrized.
        }.
 
   Definition pRegsToT (r: Kami.Semantics.RegsT): option pst :=
-    (mlet pinit: Bool <- r |> "pinit" <| None;
-       if pinit
-       then (mlet pcv: (Pc iaddrSize) <- r |> "pc" <| None;
-               mlet rfv: (Vector (Data dataBytes) rfIdx) <- r |> "rf" <| None;
-               mlet pgmv: (Vector (Data instBytes) iaddrSize) <- r |> "pgm" <| None;
-               mlet memv: (Vector (Data dataBytes) addrSize) <- r |> "mem" <| None;
-               (Some {| pc := pcv;
-                        rf := rfv;
-                        pgm := pgmv;
-                        mem := memv |}))
-       else None)%mapping.
+    (mlet pcv: (Pc iaddrSize) <- r |> "pc" <| None;
+       mlet rfv: (Vector (Data dataBytes) rfIdx) <- r |> "rf" <| None;
+       mlet pgmv: (Vector (Data instBytes) iaddrSize) <- r |> "pgm" <| None;
+       mlet memv: (Vector (Data dataBytes) addrSize) <- r |> "mem" <| None;
+       (Some {| pc := pcv; rf := rfv; pgm := pgmv; mem := memv |}))%mapping.
 
   (** * Inverting Kami rules for instruction executions *)
 
   Local Definition iaddrSizeZ: Z := Z.of_nat iaddrSize.
+
+  Ltac kinvert_more :=
+    kinvert;
+    try (repeat
+           match goal with
+           | [H: annot ?klbl = Some _ |- _] => rewrite H in *
+           | [H: (_ :: _)%struct = (_ :: _)%struct |- _] =>
+             inversion H; subst; clear H
+           end; discriminate).
 
   Lemma invert_Kami_execLd_memory:
     forall km1 kt1 kupd klbl,
@@ -75,13 +60,10 @@ Section Parametrized.
       klbl.(annot) = Some (Some "execLd"%string) ->
       exists curInst ldAddr,
         curInst = (pgm kt1) (split2 _ _ (pc kt1)) /\
-        ldAddr =
-        evalExpr
-          (alignAddr
-             _ (evalExpr
-                  (calcLdAddr
-                     _ (evalExpr (getLdAddr _ curInst))
-                     (rf kt1 (evalExpr (getLdSrc _ curInst)))))) /\
+        ldAddr = evalExpr
+                   (calcLdAddr
+                      _ (evalExpr (getLdAddr _ curInst))
+                      (rf kt1 (evalExpr (getLdSrc _ curInst)))) /\
         (evalExpr (isMMIO _ ldAddr) = false ->
          exists kt2,
            klbl.(calls) = FMap.M.empty _ /\
@@ -96,32 +78,23 @@ Section Parametrized.
                     mem := mem kt1 |}).
   Proof.
     intros.
-    kinvert; try (repeat
-                    match goal with
-                    | [H: annot ?klbl = Some _ |- _] => rewrite H in *
-                    | [H: (_ :: _)%struct = (_ :: _)%struct |- _] =>
-                      inversion H; subst; clear H
-                    end; discriminate).
+    kinvert_more.
     do 2 eexists; repeat split.
     kinv_action_dest.
     - unfold pRegsToT in *.
       kregmap_red.
-      destruct (FMap.M.find "mem"%string km1)
-        as [[[kind|] memv]|]; try discriminate.
-      destruct (decKind kind _); try discriminate.
+      destruct (FMap.M.find "mem"%string km1) as [[[memk|] memv]|]; try discriminate.
+      destruct (decKind memk _); try discriminate.
       kregmap_red.
       inversion H; subst; clear H.
       simpl in *.
-      clear -H3 Heqic.
-      congruence.
+      exfalso; clear -H3 Heqic; congruence.
     - kinv_red.
       unfold pRegsToT in *.
       kregmap_red.
       inversion H; subst; clear H; simpl in *.
-      eexists; split; [|split].
-      + assumption.
-      + reflexivity.
-      + reflexivity.
+      repeat esplit.
+      assumption.
   Qed.
 
   Lemma invert_Kami_execNm:
@@ -135,7 +108,7 @@ Section Parametrized.
         exists curInst execVal,
           curInst = (pgm kt1) (split2 _ _ (pc kt1)) /\
           execVal = evalExpr
-                      (exec
+                      (doExec
                          _
                          (rf kt1 (evalExpr (getSrc1 _ curInst)))
                          (rf kt1 (evalExpr (getSrc2 _ curInst)))
@@ -150,31 +123,26 @@ Section Parametrized.
                    mem := mem kt1 |}.
   Proof.
     intros.
-    kinvert; try (repeat
-                    match goal with
-                    | [H: annot ?klbl = Some _ |- _] => rewrite H in *
-                    | [H: (_ :: _)%struct = (_ :: _)%struct |- _] =>
-                      inversion H; subst; clear H
-                    end; discriminate).
+    kinvert_more.
     kinv_action_dest.
     unfold pRegsToT in *.
     kregmap_red.
-    destruct (FMap.M.find "mem"%string km1)
-      as [[[kind|] memv]|]; try discriminate.
-    destruct (decKind kind _); try discriminate.
+    destruct (FMap.M.find "mem"%string km1) as [[[memk|] memv]|]; try discriminate.
+    destruct (decKind memk _); try discriminate.
     kregmap_red.
     inversion H; subst; clear H.
     repeat esplit.
     assumption.
   Qed.
-  
+
 End Parametrized.
 
 Definition width: Z := 32.
 Definition width_cases: width = 32 \/ width = 64 := or_introl eq_refl.
 Local Notation nwidth := (Z.to_nat width).
 
-Definition isMMIO: IsMMIOT nwidth := cheat _.
+Instance rv32MMIO: AbsMMIO nwidth :=
+  {| isMMIO := cheat _ |}.
 
 Section PerInstAddr.
   Context {instrMemSizeLg: Z}.
@@ -188,13 +156,7 @@ Section PerInstAddr.
     (#ppc + $4)%kami_expr.
 
   Definition procInl :=
-    pprocInl
-      rv32GetOptype rv32GetLdDst (rv32GetLdAddr _) rv32GetLdSrc (rv32CalcLdAddr _)
-      (rv32GetStAddr _) rv32GetStSrc (rv32CalcStAddr _) rv32GetStVSrc
-      rv32GetSrc1 rv32GetSrc2 rv32GetDst (rv32Exec _)
-      (rv32NextPc _) (rv32AlignAddr _)
-      isMMIO procInit.
-
+    pprocInl rv32Fetch (rv32Dec _) (rv32Exec _) rv32MMIO procInit.
   Definition proc: Kami.Syntax.Modules := projT1 procInl.
 
   Definition hst := Kami.Semantics.RegsT.
@@ -209,12 +171,7 @@ Section PerInstAddr.
   (** Refinement from [p4mm] to [proc] (as a spec) *)
 
   Definition p4mm: Kami.Syntax.Modules :=
-    p4mm 1 rv32GetOptype
-         rv32GetLdDst (rv32GetLdAddr _) rv32GetLdSrc (rv32CalcLdAddr _)
-         (rv32GetStAddr _) rv32GetStSrc (rv32CalcStAddr _) rv32GetStVSrc
-         rv32GetSrc1 rv32GetSrc2 rv32GetDst (rv32Exec _)
-         (rv32NextPc _) (rv32AlignAddr _)
-         predictNextPc isMMIO procInit.
+    p4mm 1 rv32Fetch (rv32Dec _) (rv32Exec _) rv32MMIO predictNextPc procInit.
 
   Theorem proc_correct: p4mm <<== proc.
   Proof.
